Added more guts to the LIST_SORT. Still problems to solve though...

theories/core/utp_expr.thy
@@ -65,6 +65,10 @@ instance ..
 
 end
 
+definition edtype_rel :: 
+  "'VALUE WF_EXPRESSION \<Rightarrow> 'VALUE UTYPE \<Rightarrow> bool" (infix ":!\<^sub>e" 50) where
+"edtype_rel e t \<equiv> \<forall>b. \<langle>e\<rangle>\<^sub>e b :! t"
+
 lemma evar_compat_intros [simp,intro]:
   "\<lbrakk> v :\<^sub>e vtype x; \<D> v \<rbrakk> \<Longrightarrow> v \<rhd>\<^sub>e x"
   "\<lbrakk> v :\<^sub>e vtype x; \<not> aux x \<rbrakk> \<Longrightarrow> v \<rhd>\<^sub>e x"
@@ -121,13 +125,10 @@ done
 definition Op1E :: "('a \<Rightarrow> 'a) \<Rightarrow> 'a WF_EXPRESSION \<Rightarrow> 'a WF_EXPRESSION" where
 "Op1E f v = Abs_WF_EXPRESSION (\<lambda> b. f (\<langle>v\<rangle>\<^sub>e b))"
 
-definition "FUNC1 a b   = {f. \<forall>x:a. f x : b}"
-definition "FUNC2 a b c = {f. \<forall>x:a. \<forall>y:b. f x y : c}"
-
 lemma Op1E_rep_eq:
-  "\<lbrakk> v :\<^sub>e a; f \<in> FUNC1 a b \<rbrakk> \<Longrightarrow> \<langle>Op1E f v\<rangle>\<^sub>e = (\<lambda> b. f (\<langle>v\<rangle>\<^sub>e b))"
+  "\<lbrakk> v :!\<^sub>e a; f \<in> FUNC1 a b \<rbrakk> \<Longrightarrow> \<langle>Op1E f v\<rangle>\<^sub>e = (\<lambda> b. f (\<langle>v\<rangle>\<^sub>e b))"
   apply (subgoal_tac "(\<lambda> b. f (\<langle>v\<rangle>\<^sub>e b)) \<in> WF_EXPRESSION")
-  apply (auto simp add:Op1E_def WF_EXPRESSION_def FUNC1_def etype_rel_def)
+  apply (auto simp add:Op1E_def WF_EXPRESSION_def FUNC1_def edtype_rel_def)
 done
 
 definition Op2E :: "('a \<Rightarrow> 'a \<Rightarrow> 'a) \<Rightarrow> 
@@ -135,9 +136,9 @@ definition Op2E :: "('a \<Rightarrow> 'a \<Rightarrow> 'a) \<Rightarrow>
 "Op2E f v1 v2 = Abs_WF_EXPRESSION (\<lambda> b. f (\<langle>v1\<rangle>\<^sub>e b) (\<langle>v2\<rangle>\<^sub>e b))"
 
 lemma Op2E_rep_eq:
-  "\<lbrakk> x :\<^sub>e a; y :\<^sub>e b; f \<in> FUNC2 a b c \<rbrakk> \<Longrightarrow> \<langle>Op2E f x y\<rangle>\<^sub>e = (\<lambda> b1. f (\<langle>x\<rangle>\<^sub>e b1) (\<langle>y\<rangle>\<^sub>e b1))"
+  "\<lbrakk> x :!\<^sub>e a; y :!\<^sub>e b; f \<in> FUNC2 a b c \<rbrakk> \<Longrightarrow> \<langle>Op2E f x y\<rangle>\<^sub>e = (\<lambda> b1. f (\<langle>x\<rangle>\<^sub>e b1) (\<langle>y\<rangle>\<^sub>e b1))"
   apply (subgoal_tac "(\<lambda> b1. f (\<langle>x\<rangle>\<^sub>e b1) (\<langle>y\<rangle>\<^sub>e b1)) \<in> WF_EXPRESSION")
-  apply (force simp add:Op2E_def WF_EXPRESSION_def FUNC2_def etype_rel_def)+
+  apply (force simp add:Op2E_def WF_EXPRESSION_def FUNC2_def edtype_rel_def)+
 done
 
 definition DefaultE :: "'VALUE UTYPE \<Rightarrow> 'VALUE WF_EXPRESSION" where
@@ -251,12 +252,12 @@ theorem LitE_type [typing]:
   by (auto simp add:LitE_rep_eq etype_rel_def typing)
 
 theorem Op1E_type [typing]:
-  "\<lbrakk> x :\<^sub>e a; f \<in> FUNC1 a b \<rbrakk> \<Longrightarrow> Op1E f x :\<^sub>e b"
-  by (auto simp add:Op1E_rep_eq etype_rel_def typing FUNC1_def)
+  "\<lbrakk> x :!\<^sub>e a; f \<in> FUNC1 a b \<rbrakk> \<Longrightarrow> Op1E f x :!\<^sub>e b"
+  by (auto simp add:Op1E_rep_eq edtype_rel_def typing FUNC1_def)
 
 theorem Op2E_type [typing]:
-  "\<lbrakk> x :\<^sub>e a; y :\<^sub>e b; f \<in> FUNC2 a b c \<rbrakk> \<Longrightarrow> Op2E f x y :\<^sub>e c"
-  by (auto simp add:Op2E_rep_eq etype_rel_def typing FUNC2_def)
+  "\<lbrakk> x :!\<^sub>e a; y :!\<^sub>e b; f \<in> FUNC2 a b c \<rbrakk> \<Longrightarrow> Op2E f x y :!\<^sub>e c"
+  by (auto simp add:Op2E_rep_eq edtype_rel_def typing FUNC2_def)
 
 theorem AppE_type [typing]:
 "\<lbrakk> f :\<^sub>e FuncType a b; \<D> f; v :\<^sub>e a \<rbrakk> \<Longrightarrow> AppE f v :\<^sub>e b"
@@ -358,11 +359,11 @@ theorem UNREST_EXPR_LitE [unrest] :
   by (simp add:LitE_rep_eq UNREST_EXPR_def)
 
 theorem UNREST_EXPR_Op1E [unrest] :
-"\<lbrakk> x :\<^sub>e a; f \<in> FUNC1 a b; UNREST_EXPR vs x \<rbrakk> \<Longrightarrow> UNREST_EXPR vs (Op1E f x)"
+"\<lbrakk> x :!\<^sub>e a; f \<in> FUNC1 a b; UNREST_EXPR vs x \<rbrakk> \<Longrightarrow> UNREST_EXPR vs (Op1E f x)"
   by (simp add:Op1E_rep_eq UNREST_EXPR_def)
 
 theorem UNREST_EXPR_Op2E [unrest] :
-"\<lbrakk> x :\<^sub>e a; y :\<^sub>e b; f \<in> FUNC2 a b c; 
+"\<lbrakk> x :!\<^sub>e a; y :!\<^sub>e b; f \<in> FUNC2 a b c; 
    UNREST_EXPR vs x; UNREST_EXPR vs y \<rbrakk> \<Longrightarrow> UNREST_EXPR vs (Op2E f x y)"
   by (auto simp add:Op2E_rep_eq UNREST_EXPR_def)
 
